A lighter implementation of global variables.

low/Globals.v
@@ -8,505 +8,111 @@ Require Export RinternalsAux.
 
 (** Global variables that are initialised once, then treated as
  * constants.  They are initialised in the file Rinit.v. **)
-(** If you add a projection here, please make sure to also add it
- * in [Globals_projections] in the same order. **)
-Record Globals := make_Globals {
-    R_AsCharacterSymbol : SExpRec_pointer ;
-    R_BaseEnv : SExpRec_pointer ;
-    R_BaseNamespaceName : SExpRec_pointer ;
-    R_BaseNamespace : SExpRec_pointer ;
-    R_BaseSymbol : SExpRec_pointer ;
-    R_BraceSymbol : SExpRec_pointer ;
-    R_Bracket2Symbol : SExpRec_pointer ;
-    R_BracketSymbol : SExpRec_pointer ;
-    R_ClassSymbol : SExpRec_pointer ;
-    R_ColonSymbol : SExpRec_pointer ;
-    R_CommentSymbol : SExpRec_pointer ;
-    R_ConnIdSymbol : SExpRec_pointer ;
-    R_DevicesSymbol : SExpRec_pointer ;
-    R_DeviceSymbol : SExpRec_pointer ;
-    R_DimNamesSymbol : SExpRec_pointer ;
-    R_DimSymbol : SExpRec_pointer ;
-    R_DollarSymbol : SExpRec_pointer ;
-    R_dot_Class : SExpRec_pointer ;
-    R_dot_defined : SExpRec_pointer ;
-    R_DotEnvSymbol : SExpRec_pointer ;
-    R_dot_GenericCallEnv : SExpRec_pointer ;
-    R_dot_GenericDefEnv : SExpRec_pointer ;
-    R_dot_Generic : SExpRec_pointer ;
-    R_dot_Group : SExpRec_pointer ;
-    R_dot_Method : SExpRec_pointer ;
-    R_dot_Methods : SExpRec_pointer ;
-    R_dot_packageName : SExpRec_pointer ;
-    R_DotsSymbol : SExpRec_pointer ;
-    R_dot_target : SExpRec_pointer ;
-    R_DoubleColonSymbol : SExpRec_pointer ;
-    R_DropSymbol : SExpRec_pointer ;
-    R_EmptyEnv : SExpRec_pointer ;
-    R_ExactSymbol : SExpRec_pointer ;
-    R_FalseValue : SExpRec_pointer ;
-    R_GlobalEnv : SExpRec_pointer ;
-    R_LevelsSymbol : SExpRec_pointer ;
-    R_LogicalNAValue : SExpRec_pointer ;
-    R_MethodsNamespace : SExpRec_pointer ;
-    R_MissingArg : SExpRec_pointer ;
-    R_ModeSymbol : SExpRec_pointer ;
-    R_NamespaceEnvSymbol : SExpRec_pointer ;
-    R_NamespaceRegistry : SExpRec_pointer ;
-    R_NamespaceSymbol : SExpRec_pointer ;
-    R_NamesSymbol : SExpRec_pointer ;
-    R_NameSymbol  : SExpRec_pointer ;
-    R_NaRmSymbol : SExpRec_pointer ;
-    R_NilValue : SExpRec_pointer ;
-    R_PackageSymbol : SExpRec_pointer ;
-    R_PreviousSymbol : SExpRec_pointer ;
-    R_QuoteSymbol : SExpRec_pointer ;
-    R_RecursiveSymbol : SExpRec_pointer ;
-    R_RowNamesSymbol : SExpRec_pointer ;
-    R_SeedsSymbol : SExpRec_pointer ;
-    R_SortListSymbol : SExpRec_pointer ;
-    R_SourceSymbol : SExpRec_pointer ;
-    R_SpecSymbol : SExpRec_pointer ;
-    R_SrcfileSymbol : SExpRec_pointer ;
-    R_SrcrefSymbol : SExpRec_pointer ;
-    R_TmpvalSymbol : SExpRec_pointer ;
-    R_TripleColonSymbol : SExpRec_pointer ;
-    R_TrueValue : SExpRec_pointer ;
-    R_TspSymbol : SExpRec_pointer ;
-    R_UnboundValue : SExpRec_pointer ;
-    R_UseNamesSymbol : SExpRec_pointer ;
-    R_WholeSrcrefSymbol : SExpRec_pointer ;
-  }.
+Inductive GlobalVariable :=
+  | R_AsCharacterSymbol
+  | R_BaseEnv
+  | R_BaseNamespaceName
+  | R_BaseNamespace
+  | R_BaseSymbol
+  | R_BraceSymbol
+  | R_Bracket2Symbol
+  | R_BracketSymbol
+  | R_ClassSymbol
+  | R_ColonSymbol
+  | R_CommentSymbol
+  | R_ConnIdSymbol
+  | R_DevicesSymbol
+  | R_DeviceSymbol
+  | R_DimNamesSymbol
+  | R_DimSymbol
+  | R_DollarSymbol
+  | R_dot_Class
+  | R_dot_defined
+  | R_DotEnvSymbol
+  | R_dot_GenericCallEnv
+  | R_dot_GenericDefEnv
+  | R_dot_Generic
+  | R_dot_Group
+  | R_dot_Method
+  | R_dot_Methods
+  | R_dot_packageName
+  | R_DotsSymbol
+  | R_dot_target
+  | R_DoubleColonSymbol
+  | R_DropSymbol
+  | R_EmptyEnv
+  | R_ExactSymbol
+  | R_FalseValue
+  | R_GlobalEnv
+  | R_LastvalueSymbol
+  | R_LevelsSymbol
+  | R_LogicalNAValue
+  | R_MethodsNamespace
+  | R_MissingArg
+  | R_ModeSymbol
+  | R_NamespaceEnvSymbol
+  | R_NamespaceRegistry
+  | R_NamespaceSymbol
+  | R_NamesSymbol
+  | R_NameSymbol 
+  | R_NaRmSymbol
+  | R_NilValue
+  | R_PackageSymbol
+  | R_PreviousSymbol
+  | R_QuoteSymbol
+  | R_RecursiveSymbol
+  | R_RowNamesSymbol
+  | R_SeedsSymbol
+  | R_SortListSymbol
+  | R_SourceSymbol
+  | R_SpecSymbol
+  | R_SrcfileSymbol
+  | R_SrcrefSymbol
+  | R_TmpvalSymbol
+  | R_TripleColonSymbol
+  | R_TrueValue
+  | R_TspSymbol
+  | R_UnboundValue
+  | R_UseNamesSymbol
+  | R_WholeSrcrefSymbol
+  .
 
+Local Instance GlobalVariable_Comparable : Comparable GlobalVariable.
+  prove_comparable_simple_inductive.
+Defined.
 
-(** We are going to update structures of type [Globals] a lot of time
- * in Module Rinit. There is unfortunately no [{o with f := v}] syntax
- * in Coq. As we are going to need it (as it helps avoid mistakes in
- * this particular case), we implement a specialised version in Ltac. **)
+Definition Globals : Type := GlobalVariable -> SExpRec_pointer.
 
-(** Here follows a list of all the projections of [Globals]. **)
-Definition Globals_projections :=
-  [ R_AsCharacterSymbol ;
-    R_BaseEnv ;
-    R_BaseNamespaceName ;
-    R_BaseNamespace ;
-    R_BaseSymbol ;
-    R_BraceSymbol ;
-    R_Bracket2Symbol ;
-    R_BracketSymbol ;
-    R_ClassSymbol ;
-    R_ColonSymbol ;
-    R_CommentSymbol ;
-    R_ConnIdSymbol ;
-    R_DevicesSymbol ;
-    R_DeviceSymbol ;
-    R_DimNamesSymbol ;
-    R_DimSymbol ;
-    R_DollarSymbol ;
-    R_dot_Class ;
-    R_dot_defined ;
-    R_DotEnvSymbol ;
-    R_dot_GenericCallEnv ;
-    R_dot_GenericDefEnv ;
-    R_dot_Generic ;
-    R_dot_Group ;
-    R_dot_Method ;
-    R_dot_Methods ;
-    R_dot_packageName ;
-    R_DotsSymbol ;
-    R_dot_target ;
-    R_DoubleColonSymbol ;
-    R_DropSymbol ;
-    R_EmptyEnv ;
-    R_ExactSymbol ;
-    R_FalseValue ;
-    R_GlobalEnv ;
-    R_LevelsSymbol ;
-    R_LogicalNAValue ;
-    R_MethodsNamespace ;
-    R_MissingArg ;
-    R_ModeSymbol ;
-    R_NamespaceEnvSymbol ;
-    R_NamespaceRegistry ;
-    R_NamespaceSymbol ;
-    R_NamesSymbol ;
-    R_NameSymbol  ;
-    R_NaRmSymbol ;
-    R_NilValue ;
-    R_PackageSymbol ;
-    R_PreviousSymbol ;
-    R_QuoteSymbol ;
-    R_RecursiveSymbol ;
-    R_RowNamesSymbol ;
-    R_SeedsSymbol ;
-    R_SortListSymbol ;
-    R_SourceSymbol ;
-    R_SpecSymbol ;
-    R_SrcfileSymbol ;
-    R_SrcrefSymbol ;
-    R_TmpvalSymbol ;
-    R_TripleColonSymbol ;
-    R_TrueValue ;
-    R_TspSymbol ;
-    R_UnboundValue ;
-    R_UseNamesSymbol ;
-    R_WholeSrcrefSymbol ].
+Definition empty_globals : Globals :=
+  fun _ => NULL.
 
-(** No projection is missing in [Globals_projections]. **)
-Lemma Globals_projections_all : forall g g',
-  (forall C, Mem C Globals_projections -> C g = C g') ->
-  g = g'.
-Proof.
-  introv F. destruct g, g'.
-  let rec t l :=
-    match l with
-    | nil => reflexivity
-    | ?C :: ?l' =>
-      forwards E: F C;
-      [ repeat constructors
-      | simpl in E; rewrite E; clear E ];
-      t l'
-    end in
-  let l := eval unfold Globals_projections in Globals_projections in
-  t l.
-Qed.
-
-
-(** The following property translates the [{o with f := v}] syntax from
- * OCaml as a property. Intuitively, we have
- * [globals_with_list g [(C1, p1);... ; (Cn, pn)] g'] if and only if
- * [g' = {g with C1 := p1, ..., Cn := pn}]. **)
-Record globals_with_list g (L : list ((Globals -> SExpRec_pointer) * SExpRec_pointer)) g' := {
-    globals_with_list_in : forall C p,
-      Mem (C, p) L ->
-      C g' = p ;
-    globals_with_list_out : forall C,
-      (forall p, ~ Mem (C, p) L) ->
-      Mem C Globals_projections ->
-      C g' = C g ;
-  }.
-
-(** The following property is an instanciation of this property for a list with one element. **)
-Record globals_with g C p g' := {
-    globals_with_in : C g' = p ;
-    globals_with_out : forall C',
-      C <> C' ->
-      Mem C' Globals_projections ->
-      C' g' = C' g
-  }.
-
-Lemma globals_with_globals_with_list : forall g g' C p,
-  globals_with g C p g' <-> globals_with_list g [(C, p)] g'.
-Proof.
-  introv. iff G; inverts G as G1 G2; constructors; try introv F M; try introv M.
-  - repeat inverts M as M. reflexivity.
-  - apply~ G1. introv E. false F. substs. constructors~.
-  - apply~ G1.
-  - apply~ G2. introv M'. repeat inverts M' as M'. false~ F.
-Qed.
-
-Lemma globals_with_list_empty : forall g g',
-  globals_with_list g nil g' <-> g = g'.
-Proof.
-  iff G.
-  - apply Globals_projections_all. introv M.
-    symmetry. applys~ globals_with_list_out G. introv M'. inverts M'.
-  - constructors.
-    + introv M. inverts M.
-    + introv F M. rewrite~ G.
-Qed.
-
-Lemma globals_with_list_transitive : forall g1 g2 g3 L1 L2 L1',
-  globals_with_list g1 L1 g2 ->
-  (forall C v, Mem (C, v) L1 -> Mem C Globals_projections) ->
-  globals_with_list g2 L2 g3 ->
-  Filter (fun C_v => ~ exists v, Mem (fst C_v, v) L2) L1 = L1' ->
-  globals_with_list g1 (L1' ++ L2) g3.
-Proof.
-  introv G1 I G2 F. rewrite <- F. clear F. constructors.
-  - introv M. rewrite Mem_app_or_eq in M. inverts M as M.
-    + forwards (M'&NE): Filter_Mem_inv M.
-      erewrite globals_with_list_out with (g := g2).
-      * erewrite globals_with_list_in.
-        -- reflexivity.
-        -- apply G1.
-        -- autos~.
-      * apply G2.
-      * rew_logic~ in NE.
-      * applys I M'.
-    + erewrite globals_with_list_in.
-      * reflexivity.
-      * apply G2.
-      * autos~.
-  - introv NM M. erewrite globals_with_list_out with (g := g2).
-    + erewrite globals_with_list_out with (g := g1).
-      * reflexivity.
-      * apply~ G1.
-      * introv M1. eapply NM. rewrite Mem_app_or_eq. left. applys Filter_Mem M1.
-        introv (v&M2). false NM. rewrite Mem_app_or_eq. right*.
-      * autos~.
-    + apply G2.
-    + introv M'. false NM. rewrite Mem_app_or_eq. right*.
-    + autos~.
-Qed.
-
-Lemma globals_with_list_transitive_step : forall g1 g2 g3 C1 v1 L2,
-  globals_with_list g1 [(C1, v1)] g2 ->
-  Mem C1 Globals_projections ->
-  (forall v, ~ Mem (C1, v) L2) ->
-  globals_with_list g2 L2 g3 ->
-  globals_with_list g1 ((C1, v1) :: L2) g3.
-Proof.
-  introv G1 M F G2. forwards~ G: globals_with_list_transitive G1 G2.
-  - introv M'. inverts M' as M'.
-    + autos~.
-    + inverts M'.
-  - rewrite Filter_cons in G. rewrite Filter_nil in G. cases_if as I.
-    + apply G.
-    + lets (v&MI): (rm I). false* F.
-Qed.
-
-(** Adds a fresh globals in the context. **)
-Ltac allocate_Globals g :=
-  refine (let g := make_Globals in _);
-  repeat refine (let g := g _ _ _ _ _ in _); (* Small optimisation. *)
-  repeat refine (let g := g _ in _).
-
-(** Solves a goal of the form [{g' | globals_with g C p g'}] with an instanciated [C]. **)
-Ltac solve_globals_with :=
-  let g := fresh "g" in
-  let D := fresh "D" in let M := fresh "M" in
-  allocate_Globals g; exists g; unfold g; constructors;
-  [ reflexivity
-  | introv D M;
-    repeat (inverts M as M;
-            [ try solve [ reflexivity
-                        | false~ D ] |]); inverts M ].
-
-(** Solves a goal of the form [{g' | globals_with_list g L g'}] with an instanciated [L]. **)
-Ltac solve_globals_with_list :=
-  let g := fresh "g" in
-  let M := fresh "M" in let NM := fresh "NM" in
-  allocate_Globals g; exists g; unfold g; constructors;
-  [ introv M; repeat (inverts M as M; [ reflexivity |]); inverts M
-  | introv NM M;
-    repeat (inverts M as M;
-            [ try solve [ reflexivity
-                        | false NM; repeat constructors ] |]); inverts M ].
+Definition GlobalsWith (g : Globals) (C : GlobalVariable) (p : SExpRec_pointer) : Globals :=
+  fun C' =>
+    ifb C = C' then p
+    else g C'.
 
 Delimit Scope globals_scope with globals.
 
-(** The following notation builds a term [g'] such that [globals_with_list g L g']. **)
-Notation "'{{!' g 'with' L '!}}'" :=
-  (proj1_sig (ltac:(solve_globals_with_list) : { g' | globals_with_list g L g' }))
-  (only parsing)
-  : globals_scope.
-
-Notation "'{{!' g 'with' C ':=' p '!}}'" :=
-  (proj1_sig (ltac:(solve_globals_with) : { g' | globals_with g C p g' }))
-  (only parsing)
-  : globals_scope.
-
 Open Scope globals.
 
-(** A dummy element of [Globals], in which all fields are mapped to [NULL]. **)
-Definition empty_globals : Globals.
-  refine (let g := make_Globals in _);
-  repeat refine (let g := g NULL in _).
-  exact g.
-Defined.
+Notation "'{{' g 'with' C ':=' p '}}'" :=
+  (GlobalsWith g C p) : globals_scope.
 
-Lemma empty_globals_projections : forall C,
-  Mem C Globals_projections ->
-  C empty_globals = NULL.
-Proof.
-  introv M. repeat (inverts M as M; [ reflexivity |]). inverts M.
-Qed.
-
-(** Solves a goal of the form [No_duplicates L], where [L] is a list
- * of projections of [Globals]. **)
-Ltac prove_no_duplicate_projections :=
-  let M := fresh "M" in let E := fresh "E" in let g := fresh "g" in
-  repeat (apply No_duplicates_cons;
-    [ abstract
-        (introv M; repeat (inverts M as M; [
-           match type of M with ?C1 = ?C2 =>
-             set (g := {{! empty_globals with C1 := proj1_sig dummy_not_NULL !}});
-             asserts E: (C1 g = C2 g); [ rewrite M; reflexivity | inverts E ]
-           end |]);
-         inverts M)
-    |]); apply No_duplicates_nil.
-
-(** The tactic above take a lot of time to compute an additionnal proof that
- * they have computed the right object. This tactic generates a copy of [g0],
- * expect that its [n]th argument (counting from 1, from the last constructor)
- * has been replaced by [p']. It then names it [g']. **)
-Ltac generate_globals_nth_change g n p' g' :=
-  let n := eval compute in n in
-  let rec aux g c :=
-    match g with
-    | make_Globals => constr:(make_Globals)
-    | ?f ?p =>
-      match c with
-      | S O =>
-        let t := aux f O in
-        constr:(t p')
-      | S ?c' =>
-        let t := aux f c' in
-        constr:(t p)
-      | O =>
-        let t := aux f O in
-        constr:(t p)
-      end
-    | ?t =>
-      let t' := eval unfold t in t in
-      let r := aux t' c in
-      constr:(r)
-    end in
-  let r := aux g n in
-  set (g' := r).
-
-(** Same as [prove_no_duplicate_projections] when applied directly on
- * [Globals_projections], but faster, and with less memory. **)
-Ltac prove_no_duplicate_projections_fast :=
-  let M := fresh "M" in let E := fresh "E" in let g := fresh "g" in
-  repeat (apply No_duplicates_cons;
-    [ abstract
-        (introv M;
-         repeat match type of M with Mem ?C1 ?l =>
-           inverts M as M; [
-           match type of M with ?C1 = ?C2 =>
-             generate_globals_nth_change empty_globals (length l) (proj1_sig dummy_not_NULL) g;
-             asserts E: (C2 g = C1 g);
-             [ rewrite M; reflexivity
-             | false proj2_sig dummy_not_NULL E ]
-           end |]
-         end;
-         inverts M)
-    |]); apply No_duplicates_nil.
-
-(** No projection appears twice in [Globals_projections]. **)
-Lemma No_duplicates_Globals_projections : No_duplicates Globals_projections.
-Proof.
-  prove_no_duplicate_projections_fast.
-Qed.
-
-
-(** The notation [{{! g with L !}}] is useful. Unfortunately, it is actually a
- * tactic, and only works if the list [L] is known at extraction time. There
- * exists a place in the module Rinit in which the list [L] is computed at
- * execution time (its projections are however known before, but it would make
- * the definition less readable that way). We here propose need something else
- * to deal with such list: having a computable equivalent of [{{! g with L !}}].
- * Note that as [{{! g with L !}}] is faster at execution time, it is still
- * preferable when possible. **)
-
-(** Like [generate_globals_nth_change], but with [n] ranging from [1] to
- * [length Globals_projections], changing the [n]th projection from the
- * beginning. If [n = 0], the change is aborted. **)
-Ltac generate_globals_nth_change_inv g n p' g' :=
-  let len := constr:(length Globals_projections) in
-  match eval compute in (S len - n) with
-  | O => set (g' := g)
-  | ?n' =>
-    generate_globals_nth_change g n' p' g'
-  end.
-
-(** Generates a new [globals] structure [g'] from [g] in which all constructors
- * whose index are in the form [k + i * 2 ^ n] have been replaced by [p']. **)
-Ltac generate_globals_diff g n k p' g' :=
-  let n2 := eval compute in (2 ^ n) in
-  let len := eval compute in (length Globals_projections) in
-  let rec aux i g :=
-    let j := eval compute in (k + i * n2) in
-    match eval compute in (S len - j) with
-    | O =>
-      set (g' := g);
-      try clear g
-    | _ =>
-      let gi := fresh "gi" in
-      generate_globals_nth_change_inv g j p' gi;
-      try clear g;
-      aux (1 + i) gi
-    end
-  in aux 0 g.
-
-Definition Globals_with (g : Globals) (C : Globals -> SExpRec_pointer) (v : SExpRec_pointer) :
-    Mem C Globals_projections ->
-    { g' | globals_with g C v g' }.
-  introv M.
-  let E := fresh "E" in
-  let M' := fresh "M" in
-  let rec aux n k :=
-    match type of M with
-    | Mem _ [?C0] =>
-      asserts E: (C = C0);
-      [ inverts M as M; [ reflexivity | inverts M ]
-      | clear M; rewrite E; solve_globals_with ]
-    | Mem _ ?l =>
-      let g := fresh "g" in
-      let n' := eval compute in (1 + n) in
-      generate_globals_diff empty_globals n' k (proj1_sig dummy_not_NULL) g;
-      destruct (decide (C g = NULL)) eqn: E; fold_bool; rew_refl in E;
-      [ (* [true] case: we are in the first list. *)
-        asserts M': (Mem C (fst (divide_list l)));
-        [ abstract (
-            repeat (inverts M as M;
-                    [ apply Mem_here
-                    | apply Mem_next;
-                      (inverts M as M; [ false proj2_sig dummy_not_NULL E |])
-                       || solve [ inverts M ] ]);
-            solve [ inverts M ])
-        | clear - M'; rename M' into M; simpl in M;
-          let k' := eval compute in (k + 2 ^ n)%nat in
-          abstract (aux n' k') ]
-      | (* [false] case: we are in the second list. *)
-        asserts M': (Mem C (snd (divide_list l)));
-        [ abstract (
-            repeat (inverts M as M;
-                    [ false~ E
-                    | (inverts M as M; [ apply Mem_here | apply Mem_next ])
-                       || solve [ inverts M ] ]);
-            solve [ inverts M ])
-      | clear - M'; rename M' into M; simpl in M;
-        let k' := eval compute in (k + 2 ^ (1 + n))%nat in
-        abstract (aux n' k') ]
-      ]
-    end
-  in aux 0 2.
-Defined.
-
-Definition Globals_with_list (g : Globals) (L : list ((Globals -> SExpRec_pointer) * SExpRec_pointer)) :
-    (forall C v, Mem (C, v) L -> Mem C Globals_projections) ->
-    No_duplicates (map fst L) ->
-    { g' | globals_with_list g L g' }.
-  introv F ND. gen g. induction L; introv.
-  - exists g. rewrite~ globals_with_list_empty.
-  - destruct a as [C v]. asserts M: (Mem C Globals_projections).
-    + apply~ F.
-    + forwards IHg: IHL (proj1_sig (Globals_with g C v M)).
-      * introv M'. apply~ F. apply* Mem_next.
-      * inverts~ ND.
-      * exists (proj1_sig IHg). apply~ globals_with_list_transitive_step.
-        -- rewrite <- globals_with_globals_with_list.
-           refine (proj2_sig (Globals_with _ _ _ M)).
-        -- introv M'. rew_list in ND. inverts ND as NM ND. false NM.
-           applys Mem_map M'.
-        -- apply~ proj2_sig.
-Defined.
-
-(** We can now prove a notation for this function. **)
-Notation "'{{' g 'with' L 'using' F ',' ND '}}'" :=
-  (proj1_sig (Globals_with_list g L F ND)) : globals_scope.
-
-(** Solves a goal of the form [forall C v, Mem (C, v) L -> Mem C Globals_projections]
- * with an instanciated [L]. **)
-Ltac prove_mem_Globals_projections :=
-  let M := fresh "M" in
-  introv M; repeat constructors.
+Definition GlobalsWith_list :=
+  fold_left (fun C_p g => GlobalsWith g (fst C_p) (snd C_p)).
 
 Notation "'{{' g 'with' L '}}'" :=
-  ({{ g with L using ltac:(prove_mem_Globals_projections),
-                     ltac:(prove_no_duplicate_projections)}})
-  (only parsing) : globals_scope.
+  (GlobalsWith_list g L) : globals_scope.
+
+
+(** To avoid too many closures. **)
+Definition flatten_Globals (g : Globals) : Globals.
+  refine (proj1_sig (_ : { g' | forall C, g C = g' C })).
+  refine (exist _ (let args : _ := _ in fun C : GlobalVariable =>
+                   ltac:(destruct C; do 100 (exact (fst args) || refine (let args := snd args in _)))) _).
+  intro C. destruct C; try reflexivity.
+  refine (exist _ (let args : _ := _ in fun C : GlobalVariable =>
+                   ltac:(destruct C; repeat (exact (fst args) || refine (let args := snd args in _)))) _).
+  intro C. destruct C; repeat (exact (fst args) || refine (let args := snd args in _)).
+Defined.
 
